more updates to stlc

stlc.v
@@ -14,11 +14,11 @@ Inductive ty : Type :=
   | TArr : ty -> ty -> ty.
 
 (* Terms *)
-Inductive tm : Type :=
-  | tvar : id -> tm
-  | tabs : id -> ty -> tm -> tm
-  | tapp : tm -> tm -> tm
-  | tnum : nat -> tm.
+Inductive exp : Type :=
+  | tvar : id -> exp
+  | tabs : id -> ty -> exp -> exp
+  | tapp : exp -> exp -> exp
+  | tnum : nat -> exp.
 
 Tactic Notation "t_cases" tactic(first) ident(c) :=
   first;
@@ -26,17 +26,15 @@ Tactic Notation "t_cases" tactic(first) ident(c) :=
   | Case_aux c "tapp" | Case_aux c "tnum" ].
 
 (* Values *)
-Inductive value : tm -> Prop :=
+Inductive value : exp -> Prop :=
   | v_abs : forall x T t, value (tabs x T t)
   | v_num : forall n, value (tnum n).
 
 Hint Constructors value.
 
-Definition context := partial_map ty.
-
-Reserved Notation "Gamma '|-' t '\in' T" (at level 40).
+Definition context := partial_map ty.  Reserved Notation "Gamma '|-' t '\in' T" (at level 40).
     
-Inductive has_type : context -> tm -> ty -> Prop :=
+Inductive has_type : context -> exp -> ty -> Prop :=
   | T_Var : forall Gamma x T,
       Gamma x = Some T ->
       Gamma |- tvar x \in T
@@ -55,15 +53,14 @@ where "Gamma '|-' t '\in' T" := (has_type Gamma t T).
 Tactic Notation "has_type_cases" tactic(first) ident(c) :=
   first;
   [ Case_aux c "T_Var" | Case_aux c "T_Abs" 
-  | Case_aux c "T_App" | Case_aux c "T_True" 
-  | Case_aux c "T_False" | Case_aux c "T_If" ].
+  | Case_aux c "T_App" | Case_aux c "T_Num" ].
 
 Hint Constructors has_type.
 
 (* Substitution *)
 Reserved Notation "'[' x ':=' s ']' t" (at level 20).
 
-Fixpoint subst (x:id) (s:tm) (t:tm) : tm :=
+Fixpoint subst (x:id) (s:exp) (t:exp) : exp :=
   match t with
   | tvar x' => 
       if eq_id_dec x x' then s else t
@@ -78,22 +75,24 @@ Fixpoint subst (x:id) (s:tm) (t:tm) : tm :=
 where "'[' x ':=' s ']' t" := (subst x s t).
 
 (* Rewriting Style Type Checking Relation *)
-Inductive exp : Type :=
-  | evar  : id -> exp
-  | eabs  : id -> ty -> exp -> exp
-  | eapp  : exp -> exp -> exp
-  | enum  : nat -> exp
-  | tearr : ty -> exp -> exp
-  | tenum : exp.
+Inductive mexp : Type :=
+  | evar  : id -> mexp
+  | eabs  : id -> ty -> mexp -> mexp
+  | eapp  : mexp -> mexp -> mexp
+  | enum  : nat -> mexp
+  | tearr : ty -> mexp -> mexp
+  | tenum : mexp.
 
-Inductive exp_type : exp -> Prop :=
-  | t_tenum : exp_type tenum
-  | t_tearr : forall t e, exp_type (tearr t e).
+Hint Constructors mexp.
 
-Fixpoint ty__exp (t : ty) : exp :=
+Inductive mexp_type : mexp -> Prop :=
+  | t_tenum : mexp_type tenum
+  | t_tearr : forall t e, mexp_type e -> mexp_type (tearr t e).
+
+Fixpoint ty__mexp (t : ty) : mexp :=
   match t with
   | TNum => tenum
-  | TArr t1 t2 => tearr t1 (ty__exp t2)
+  | TArr t1 t2 => tearr t1 (ty__mexp t2)
   end.
 
 Fixpoint beq_ty (t1 : ty) (t2 : ty) : bool :=
@@ -103,30 +102,45 @@ Fixpoint beq_ty (t1 : ty) (t2 : ty) : bool :=
   | _,_ => false
   end.
 
-Fixpoint beq_ty_exp (t : ty) (e : exp) : bool :=
+Fixpoint beq_ty_mexp (t : ty) (e : mexp) : bool :=
   match t, e with
   | TNum, tenum => true
-  | TArr t1 t2, tearr t1' t2' => beq_ty t1 t1' && beq_ty_exp t2 t2'
+  | TArr t1 t2, tearr t1' t2' => beq_ty t1 t1' && beq_ty_mexp t2 t2'
   | _,_ => false
   end.
 
-Example beq_ty_exp_ex1 :
-  beq_ty_exp TNum tenum = true.
+Fixpoint inj (e : exp) : mexp :=
+  match e with
+  | tvar x      => evar x
+  | tabs x t e' => eabs x t (inj e')
+  | tapp e1 e2  => eapp (inj e1) (inj e2)
+  | tnum n      => enum n
+  end.
+
+Fixpoint proj (m : mexp) : option ty :=
+  match m with
+  | tearr t m' => option_map (TArr t) (proj m')
+  | tenum      => Some TNum
+  | _          => None
+  end.
+
+Example beq_ty_mexp_ex1 :
+  beq_ty_mexp TNum tenum = true.
 Proof. reflexivity. Qed.
 
-Example beq_ty_exp_ex2 :
-  beq_ty_exp (TArr TNum TNum) (tearr TNum tenum) = true.
+Example beq_ty_mexp_ex2 :
+  beq_ty_mexp (TArr TNum TNum) (tearr TNum tenum) = true.
 Proof. reflexivity. Qed.
 
-Example beq_ty_exp_ex3 :
-  beq_ty_exp (TArr (TArr TNum TNum) TNum) (tearr (TArr TNum TNum) tenum) = true.
+Example beq_ty_mexp_ex3 :
+  beq_ty_mexp (TArr (TArr TNum TNum) TNum) (tearr (TArr TNum TNum) tenum) = true.
 Proof. reflexivity. Qed.
 
 Reserved Notation "'{' x ':=' s '}' t" (at level 20).
 
-Fixpoint subst_exp (x:id) (s:ty) (t:exp) : exp :=
+Fixpoint subst_mexp (x:id) (s:ty) (t:mexp) : mexp :=
   match t with
-  | evar x'     => if eq_id_dec x x' then ty__exp s else evar x'
+  | evar x'     => if eq_id_dec x x' then ty__mexp s else evar x'
   | eabs x' T e => eabs x' T (if eq_id_dec x x' then e else ({x:=s} e))
   | eapp e1 e2  => eapp ({x:=s} e1) ({x:=s} e2)
   | enum n      => enum n
@@ -134,31 +148,78 @@ Fixpoint subst_exp (x:id) (s:ty) (t:exp) : exp :=
   | tenum       => tenum
   end
 
-where "'{' x ':=' s '}' t" := (subst_exp x s t).
+where "'{' x ':=' s '}' t" := (subst_mexp x s t).
 
 Reserved Notation "e1 '==>' e2" (at level 40).
 
-Inductive rewrite : exp -> exp -> Prop :=
-  | tcnum  : forall n, enum n ==> tenum
-  | tcabs  : forall x t eh, eabs x t eh ==> tearr t ({x:=t} eh)
-  | tctb   : forall t1 t1' t2, beq_ty_exp t1 t1' = true -> eapp (tearr t1 t2) t1' ==> t2
-  | tcapp1 : forall e1 e1' e2, e1 ==> e1' -> eapp e1 e2 ==> eapp e1' e2
-  | tcapp2 : forall t1 e2 e2', exp_type t1 -> e2 ==> e2' -> eapp t1 e2 ==> eapp t1 e2'
-  | tcarr  : forall t1 e2 e2', e2 ==> e2' -> tearr t1 e2 ==> tearr t1 e2'
+Inductive rewrite : mexp -> mexp -> Prop :=
+  | tcnum  : forall n,
+      enum n ==> tenum
+  | tcabs  : forall x t eh,
+      eabs x t eh ==> tearr t ({x:=t} eh)
+  | tctb   : forall t1 t1' t2,
+      beq_ty_mexp t1 t1' = true ->
+      eapp (tearr t1 t2) t1' ==> t2
+  | tcapp1 : forall e1 e1' e2,
+      e1 ==> e1' ->
+      eapp e1 e2 ==> eapp e1' e2
+  | tcapp2 : forall t1 e2 e2',
+      mexp_type t1 ->
+      e2 ==> e2' ->
+      eapp t1 e2 ==> eapp t1 e2'
+  | tcarr  : forall t1 e2 e2',
+      e2 ==> e2' ->
+      tearr t1 e2 ==> tearr t1 e2'
 
 where "e1 '==>' e2" := (rewrite e1 e2).
+
+Hint Constructors rewrite.
 
 Notation multirewrite := (multi rewrite).
 Notation "e1 '==>*' e2" := (multirewrite e1 e2) (at level 40).
 
-(* I need a more powerful representation of exp... *)
-Theorem rewrite_sound : forall e t t',
-  empty |- e \in t -> e ==>* t' /\ beq_ty_exp t t'.
+Theorem rewrite_sound : forall e t,
+  empty |- e \in t ->
+    exists m, inj e ==>* m /\ proj m = Some t.
 Proof.
+  intros e t Ht.
+  has_type_cases (induction Ht) Case.
+  Case "T_Var".
+    admit.
+  Case "T_Abs".
+    inversion IHHt. inversion H.
+    exists (tearr T11 x0).
+    split; subst.
+    SCase "left".
+      simpl.
+      eapply multi_step. apply tcabs.
+      eapply multi_step. apply tcarr.
+      inversion IHHt.
+      inversion H2.
+      inversion H3; subst.
+        destruct (inj t12); try (solve by inversion).
+          simpl. 
+
+      inversion H0; subst.
+        destruct ({x:=T11}inj t12).
+
+  t_cases (induction e) Case;
+    inversion Ht; subst.
+  Case "tvar".
+    inversion H1.
+  Case "tabs".
+    assert (exists t1, proj t1 = Some T12).
+      admit.
+    inversion H; subst.
+    exists (tearr t0 x).
+    split.
+      simpl.
+
 Admitted.
 
-Theorem rewrite_complete : forall e t,
-  e ==>* t -> empty |- e \in t.
+Theorem rewrite_complete : forall e m,
+  inj e ==>* m ->
+    exists t, empty |- e \in t /\ proj m = Some t.
 Proof.
 Admitted.
 
