stlc2.v
@@ -1,0 +1,272 @@
+(* stlc.v *)
+
+Require Export SfLib.
+
+(* formalization of the simply typed lambda calculus, coq fixpoint declaration
+   for the rewriting semantics, and proof of the soundness and completenes of
+   the rewriting semantics to the type system described in the stlc
+   formalization
+*)
+
+(* Rewriting Style Type Checking Relation *)
+Inductive mexp : Type :=
+  | evar : id -> mexp
+  | eabs : id -> mexp -> mexp -> mexp
+  | eapp : mexp -> mexp -> mexp
+  | enum : nat -> mexp
+  | tarr : mexp -> mexp -> mexp
+  | tnum : mexp.
+
+Hint Constructors mexp.
+
+Tactic Notation "mexp_cases" tactic(first) ident(c) :=
+  first;
+  [ Case_aux c "evar" | Case_aux c "eabs" 
+  | Case_aux c "eapp" | Case_aux c "enum"
+  | Case_aux c "tarr" | Case_aux c "tnum" ].
+
+(*
+Fixpoint beq_mexp (e1 e2 : mexp) : bool :=
+  match e1, e2 with
+  | evar i1, evar i2 => eq_id_dec i1 i2
+  | eabs i1 t1 m1, eabs i2 t2 m2 => 
+      andb (andb (eq_id_dec i1 i2)
+                 (beq_mexp t1 t2))
+           (beq_mexp m1 m2)
+  | eapp m1 n1, eapp m2 n2 => andb (beq_mexp m1 m2) (beq_mexp n1 n2)
+  | enum n1, enum n2 => beq_nat n1 n2
+  | tarr s1 t1, tarr s2 t2 => andb (beq_mexp s1 s2) (beq_mexp t1 t2)
+  | tnum, tnum => true
+  | _,_ => false
+  end.
+*)
+
+Inductive type : mexp -> Prop :=
+  | t_tnum : type tnum
+  | t_tarr : forall e1 e2, type e1 -> type e2 -> type (tarr e1 e2).
+
+Hint Constructors type.
+
+Inductive exp : mexp -> Prop :=
+  | e_evar : forall x, exp (evar x)
+  | e_eabs : forall x t e, type t -> exp e -> exp (eabs x t e)
+  | e_eapp : forall e1 e2, exp e1 -> exp e2 -> exp (eapp e1 e2)
+  | e_enum : forall n, exp (enum n).
+
+Hint Constructors exp.
+
+Inductive value : mexp -> Prop :=
+  | v_eabs : forall x t e, type t -> exp e -> value (eabs x t e)
+  | v_enum : forall n, value (enum n).
+
+Hint Constructors value.
+
+Definition context := partial_map mexp.
+
+Reserved Notation "Gamma '|-' t '\in' T" (at level 40).
+    
+Inductive has_type : context -> mexp -> mexp -> Prop :=
+  | T_Var : forall Gamma x t,
+      type t ->
+      Gamma x = Some t ->
+      Gamma |- evar x \in t
+  | T_Abs : forall Gamma x xt e et,
+      type xt -> type et -> exp e ->
+      extend Gamma x xt |- e \in et ->
+      Gamma |- eabs x xt e \in tarr xt et
+  | T_App : forall Gamma e1 e2 t11 t12,
+      exp e1 -> exp e2 -> type t11 -> type t12 ->
+      Gamma |- e1 \in tarr t11 t12 ->
+      Gamma |- e2 \in t11 ->
+      Gamma |- eapp e1 e2 \in t12
+  | T_Num : forall Gamma n,
+      Gamma |- enum n \in tnum
+
+where "Gamma '|-' t '\in' T" := (has_type Gamma t T).
+
+Tactic Notation "has_type_cases" tactic(first) ident(c) :=
+  first;
+  [ Case_aux c "T_Var" | Case_aux c "T_Abs" 
+  | Case_aux c "T_App" | Case_aux c "T_Num" ].
+
+Hint Constructors has_type.
+
+Reserved Notation "'{' x ':=' s '}' t" (at level 20).
+
+Fixpoint subst (x:id) (s:mexp) (t:mexp) : mexp :=
+  match t with
+  | evar x'     => if eq_id_dec x x' then s else evar x'
+  | eabs x' t e => eabs x' t (if eq_id_dec x x' then e else ({x:=s} e))
+  | eapp e1 e2  => eapp ({x:=s} e1) ({x:=s} e2)
+  | enum n      => enum n
+  | tarr t1 t2  => tarr t1 t2
+  | tnum        => tnum
+  end
+
+where "'{' x ':=' s '}' t" := (subst x s t).
+
+Reserved Notation "e1 '==>' e2" (at level 40).
+
+Inductive rewrite : mexp -> mexp -> Prop :=
+  | tcnum  : forall n,
+      enum n ==> tnum
+  | tcabs  : forall x t eh,
+      eabs x t eh ==> tarr t ({x:=t} eh)
+  | tctb   : forall t1 t2,
+      eapp (tarr t1 t2) t1 ==> t2
+  | tcapp1 : forall e1 e1' e2,
+      e1 ==> e1' ->
+      eapp e1 e2 ==> eapp e1' e2
+  | tcapp2 : forall t1 e2 e2',
+      type t1 ->
+      e2 ==> e2' ->
+      eapp t1 e2 ==> eapp t1 e2'
+  | tcarr  : forall t1 e2 e2',
+      type t1 ->
+      e2 ==> e2' ->
+      tarr t1 e2 ==> tarr t1 e2'
+
+where "e1 '==>' e2" := (rewrite e1 e2).
+
+Tactic Notation "rewrite_cases" tactic(first) ident(c) :=
+  first;
+  [ Case_aux c "tcnum" | Case_aux c "tcabs" 
+  | Case_aux c "tctb" | Case_aux c "tcapp1" 
+  | Case_aux c "tcapp2" | Case_aux c "tcarr" ].
+
+Hint Constructors rewrite.
+
+Notation multirewrite := (multi rewrite).
+Notation "e1 '==>*' e2" := (multirewrite e1 e2) (at level 40).
+
+Inductive appears_free_in : id -> mexp -> Prop :=
+  | afi_var : forall x,
+      appears_free_in x (evar x)
+  | afi_app1 : forall x e1 e2,
+      appears_free_in x e1 ->
+      appears_free_in x (eapp e1 e2)
+  | afi_app2 : forall x e1 e2,
+      appears_free_in x e2 ->
+      appears_free_in x (eapp e1 e2)
+  | afi_abs : forall x y ty e,
+      y <> x ->
+      appears_free_in x e ->
+      appears_free_in x (eabs y ty e).
+
+Tactic Notation "afi_cases" tactic(first) ident(c) :=
+  first;
+  [ Case_aux c "afi_var"  | Case_aux c "afi_app1"
+  | Case_aux c "afi_app2" | Case_aux c "afi_abs" ].
+
+Hint Constructors appears_free_in.
+
+Definition closed (e:mexp) :=
+  forall x, ~ appears_free_in x e.
+
+Lemma free_in_context : forall x e t Gamma,
+   appears_free_in x e ->
+   Gamma |- e \in t ->
+   exists t', Gamma x = Some t'.
+Proof. Admitted.
+
+Lemma context_invariance : forall Gamma Gamma' e t,
+     Gamma |- e \in t  ->
+     (forall x, appears_free_in x e -> Gamma x = Gamma' x) ->
+     Gamma' |- e \in t.
+Proof. Admitted.
+
+Lemma substitution_preserves_typing : forall Gamma x tx e v te,
+     extend Gamma x tx |- e \in te ->
+     empty |- v \in tx   ->
+     Gamma |- {x:=v}e \in te.
+Proof. Admitted.
+
+Theorem rewrite_progress : forall e t,
+  empty |- e \in t ->
+  type e \/ exists e', e ==> e'.
+Proof. Admitted.
+
+Theorem rewrite_sound : forall e t,
+  empty |- e \in t -> e ==>* t.
+Proof.
+Admitted.
+(*
+  intros e t Ht.
+  has_type_cases (induction Ht) Case.
+  Case "T_Var".
+    admit. (* This case would be covered if I still had Ht *)
+  Case "T_Abs".
+    eapply multi_step. eapply tcabs.
+    eapply multi_step. eapply tcarr.
+      assumption.
+
+
+  mexp_cases (induction e) Case;
+    inversion Ht; subst.
+  Case "evar". inversion H2.
+  Case "eabs".
+    eapply multi_step. eapply tcabs.
+    eapply multi_step. eapply tcarr.
+      assumption.
+*)
+
+      
+
+Theorem rewrite_complete : forall e t,
+  exp e -> type t ->
+  e ==>* t ->
+  empty |- e \in t.
+Proof. Admitted.
+
+Theorem rewrite_type_equiv : forall e t,
+  empty |- e \in t <-> e ==>* t.
+Proof.
+  split.
+    apply rewrite_sound.
+    apply rewrite_complete.
+Qed.
+
+
+Inductive eval : mexp -> mexp -> Prop :=
+  | eval_app1 : forall e1 e1' e2,
+      eval e1 e1' ->
+      eval (eapp e1 e2) (eapp e1' e2)
+  | eval_app2 : forall v1 e2 e2',
+      value v1 ->
+      eval e2 e2' ->
+      eval (eapp v1 e2) (eapp v1 e2')
+  | eval_app : forall x xt e v,
+      value v ->
+      eval (eapp (eabs x xt e) v) ({x:=v} e)
+  .
+
+Inductive arrow : mexp -> mexp -> Prop :=
+  | arrow_rewrite : forall e1 e2,
+      e1 ==> e2 ->
+      arrow e1 e2
+  | arrow_eval    : forall e1 e2,
+      eval e1 e2 ->
+      arrow e1 e2
+  .
+
+(*
+Theorem non_confluence_of_arrow : exists e eh eh',
+  arrow e eh /\ arrow e eh' /\ beq_mexp eh eh' = false.
+Proof.
+Admitted.
+*)
+
+Theorem preservation : forall e e' t,
+  type t ->
+  e ==>* t ->
+  eval e e' ->
+  e' ==>* t.
+Proof. Admitted.
+
+Theorem progress : forall e e' t,
+  e ==>* t ->
+
+
+
+
+
